`StateGettersEquivalence`: add `TIMESTAMP` equivalence proof

EvmEquivalence/Equivalence/StateGettersEquivalence.lean
@@ -18,6 +18,7 @@ inductive stateGetter_op where
   | caller
   | gasprice
   | coinbase
+  | timestamp
 
 variable (op : stateGetter_op)
 
@@ -28,6 +29,7 @@ def stateGetter_op.to_binop : stateGetter_op → SortNullStackOp
   | .caller => .CALLER_EVM_NullStackOp
   | .gasprice => .GASPRICE_EVM_NullStackOp
   | .coinbase => .COINBASE_EVM_NullStackOp
+  | .timestamp => .TIMESTAMP_EVM_NullStackOp
 
 def stateGetter_op.from_k : stateGetter_op → StateGettersSummary.stateGetter_op
  | .address  => .address
@@ -35,9 +37,10 @@ def stateGetter_op.from_k : stateGetter_op → StateGettersSummary.stateGetter_o
  | .caller => .caller
  | .gasprice => .gasprice
  | .coinbase => .coinbase
+ | .timestamp => .timestamp
 
 def oneOpLHS
-  {GAS_CELL ID_CELL ORIGIN_CELL CALLER_CELL COINBASE_CELL PC_CELL _Val6 _Val8 : SortInt}
+  {GAS_CELL ID_CELL ORIGIN_CELL CALLER_CELL COINBASE_CELL TIMESTAMP_CELL PC_CELL _Val6 _Val8 : SortInt}
   -- We assume `GASPRICE_CELL` is not negative
   {GASPRICE_CELL : ℕ}
   {SCHEDULE_CELL : SortSchedule}
@@ -100,13 +103,14 @@ def oneOpLHS
           origin := { val := (@inj SortInt SortAccount) ORIGIN_CELL },
           blockhashes := _Gen19,
           block := {_Gen20 with
-                    coinbase := { val := COINBASE_CELL}
+                    coinbase := { val := COINBASE_CELL},
+                    timestamp := { val := TIMESTAMP_CELL }
                     } },
         network := _DotVar2 } },
     generatedCounter := _DotVar0 }
 
 def oneOpRHS
-  {TOP_STACK ID_CELL ORIGIN_CELL CALLER_CELL COINBASE_CELL _Val6 _Val8 : SortInt}
+  {TOP_STACK ID_CELL ORIGIN_CELL CALLER_CELL COINBASE_CELL TIMESTAMP_CELL _Val6 _Val8 : SortInt}
   -- We assume `GASPRICE_CELL` is not negative
   {GASPRICE_CELL : ℕ}
   {SCHEDULE_CELL : SortSchedule}
@@ -168,7 +172,8 @@ def oneOpRHS
             origin := { val := (@inj SortInt SortAccount) ORIGIN_CELL },
             blockhashes := _Gen19,
             block := {_Gen20 with
-                    coinbase := { val := COINBASE_CELL}
+                    coinbase := { val := COINBASE_CELL},
+                    timestamp := { val := TIMESTAMP_CELL }
                     } },
           network := _DotVar2 } },
       generatedCounter := _DotVar0 }
@@ -190,9 +195,10 @@ def stateGetter_op.do (tc : SortGeneratedTopCell) : SortInt :=
   | .caller => acc2Int tc.caller.val
   | .gasprice => Int.toNat tc.gasPrice.val
   | .coinbase => tc.coinbase.val
+  | .timestamp => tc.timestamp.val
 
 theorem rw_oneOpLHS_oneOpRHS
-  {GAS_CELL ID_CELL ORIGIN_CELL CALLER_CELL COINBASE_CELL PC_CELL _Val0 _Val2 _Val6 _Val7 _Val8 : SortInt}
+  {GAS_CELL ID_CELL ORIGIN_CELL CALLER_CELL COINBASE_CELL TIMESTAMP_CELL PC_CELL _Val0 _Val2 _Val6 _Val7 _Val8 : SortInt}
   -- We assume `GASPRICE_CELL` is not negative
   {GASPRICE_CELL : ℕ}
   {SCHEDULE_CELL : SortSchedule}
@@ -232,10 +238,10 @@ theorem rw_oneOpLHS_oneOpRHS
   (defn_Val7 : «_<_>_SCHEDULE_Int_ScheduleConst_Schedule» SortScheduleConst.Gbase_SCHEDULE_ScheduleConst SCHEDULE_CELL = some _Val7)
   (defn_Val8 : «_-Int_» GAS_CELL _Val7 = some _Val8)
   (req : _Val5 = true):
-  let lhs := (@oneOpLHS op GAS_CELL ID_CELL ORIGIN_CELL CALLER_CELL COINBASE_CELL PC_CELL _Val6 _Val8 GASPRICE_CELL SCHEDULE_CELL USEGAS_CELL WS _DotVar0 _DotVar2 _Gen0 _Gen1 _Gen10
+  let lhs := (@oneOpLHS op GAS_CELL ID_CELL ORIGIN_CELL CALLER_CELL COINBASE_CELL TIMESTAMP_CELL PC_CELL _Val6 _Val8 GASPRICE_CELL SCHEDULE_CELL USEGAS_CELL WS _DotVar0 _DotVar2 _Gen0 _Gen1 _Gen10
   _Gen11 _Gen12 _Gen13 _Gen14 _Gen15 _Gen16 _Gen19
   _Gen20 _Gen21 _Gen22 _Gen3 _Gen4 _Gen5 _Gen6 _Gen7 _Gen8 _Gen9 _K_CELL)
-  let rhs := (@oneOpRHS (op.do lhs) ID_CELL ORIGIN_CELL CALLER_CELL COINBASE_CELL _Val6 _Val8 GASPRICE_CELL SCHEDULE_CELL WS _DotVar0 _DotVar2 _Gen0 _Gen1 _Gen10 _Gen11 _Gen12 _Gen13 _Gen14 _Gen15 _Gen16 _Gen19 _Gen20 _Gen21 _Gen22 _Gen3 _Gen4 _Gen5 _Gen6 _Gen7 _Gen8 _Gen9 _K_CELL)
+  let rhs := (@oneOpRHS (op.do lhs) ID_CELL ORIGIN_CELL CALLER_CELL COINBASE_CELL TIMESTAMP_CELL _Val6 _Val8 GASPRICE_CELL SCHEDULE_CELL WS _DotVar0 _DotVar2 _Gen0 _Gen1 _Gen10 _Gen11 _Gen12 _Gen13 _Gen14 _Gen15 _Gen16 _Gen19 _Gen20 _Gen21 _Gen22 _Gen3 _Gen4 _Gen5 _Gen6 _Gen7 _Gen8 _Gen9 _K_CELL)
   Rewrites lhs rhs
    := by
   --intro lhs rhs; simp [lhs, rhs, oneOpLHS, oneOpRHS]
@@ -250,9 +256,11 @@ theorem rw_oneOpLHS_oneOpRHS
     <;> try assumption
   . apply (@Rewrites.COINBASE_SUMMARY_COINBASE_SUMMARY_USEGAS COINBASE_CELL GAS_CELL PC_CELL _Val0 _Val2)
     <;> try assumption
+  . apply (@Rewrites.TIMESTAMP_SUMMARY_TIMESTAMP_SUMMARY_USEGAS GAS_CELL PC_CELL TIMESTAMP_CELL _Val0 _Val2)
+    <;> try assumption
 
 theorem oneOp_prestate_equiv
-  {GAS_CELL ID_CELL ORIGIN_CELL CALLER_CELL COINBASE_CELL PC_CELL _Val6 _Val8 : SortInt}
+  {GAS_CELL ID_CELL ORIGIN_CELL CALLER_CELL COINBASE_CELL TIMESTAMP_CELL PC_CELL _Val6 _Val8 : SortInt}
   -- We assume `GASPRICE_CELL` is not negative
   {GASPRICE_CELL : ℕ}
   {SCHEDULE_CELL : SortSchedule}
@@ -282,7 +290,7 @@ theorem oneOp_prestate_equiv
   {_Gen9 : SortCallDepthCell}
   {_K_CELL : SortK}
   (symState : EVM.State):
-  let lhs := (@oneOpLHS op GAS_CELL ID_CELL ORIGIN_CELL CALLER_CELL COINBASE_CELL PC_CELL _Val6 _Val8 GASPRICE_CELL SCHEDULE_CELL USEGAS_CELL WS _DotVar0 _DotVar2 _Gen0 _Gen1 _Gen10
+  let lhs := (@oneOpLHS op GAS_CELL ID_CELL ORIGIN_CELL CALLER_CELL COINBASE_CELL TIMESTAMP_CELL PC_CELL _Val6 _Val8 GASPRICE_CELL SCHEDULE_CELL USEGAS_CELL WS _DotVar0 _DotVar2 _Gen0 _Gen1 _Gen10
   _Gen11 _Gen12 _Gen13 _Gen14 _Gen15 _Gen16 _Gen19
   _Gen20 _Gen21 _Gen22 _Gen3 _Gen4 _Gen5 _Gen6 _Gen7 _Gen8 _Gen9 _K_CELL)
   stateMap symState lhs =
@@ -311,7 +319,7 @@ theorem oneOp_prestate_equiv
     simp [oneOpLHS, cop, stateMap, stateGetter_op.from_k] <;> rfl
 
 theorem oneOp_poststate_equiv
-  {TOP_STACK ID_CELL ORIGIN_CELL CALLER_CELL COINBASE_CELL PC_CELL _Val5 _Val6 _Val8 : SortInt}
+  {TOP_STACK ID_CELL ORIGIN_CELL CALLER_CELL COINBASE_CELL TIMESTAMP_CELL PC_CELL _Val5 _Val6 _Val8 : SortInt}
   -- We assume `GASPRICE_CELL` is not negative
   {GASPRICE_CELL : ℕ}
   {SCHEDULE_CELL : SortSchedule}
@@ -341,7 +349,7 @@ theorem oneOp_poststate_equiv
   {_K_CELL : SortK}
   (defn_Val6 : «_+Int_» PC_CELL 1 = some _Val6)
   (symState : EVM.State):
-  let rhs := (@oneOpRHS TOP_STACK ID_CELL ORIGIN_CELL CALLER_CELL COINBASE_CELL _Val6 _Val8 GASPRICE_CELL SCHEDULE_CELL WS _DotVar0 _DotVar2 _Gen0 _Gen1 _Gen10 _Gen11 _Gen12 _Gen13 _Gen14 _Gen15 _Gen16 _Gen19 _Gen20 _Gen21 _Gen22 _Gen3 _Gen4 _Gen5 _Gen6 _Gen7 _Gen8 _Gen9 _K_CELL)
+  let rhs := (@oneOpRHS TOP_STACK ID_CELL ORIGIN_CELL CALLER_CELL COINBASE_CELL TIMESTAMP_CELL _Val6 _Val8 GASPRICE_CELL SCHEDULE_CELL WS _DotVar0 _DotVar2 _Gen0 _Gen1 _Gen10 _Gen11 _Gen12 _Gen13 _Gen14 _Gen15 _Gen16 _Gen19 _Gen20 _Gen21 _Gen22 _Gen3 _Gen4 _Gen5 _Gen6 _Gen7 _Gen8 _Gen9 _K_CELL)
   stateMap symState rhs =
   {symState with
     stack := (intMap TOP_STACK) :: wordStackMap WS
@@ -376,7 +384,7 @@ attribute [local simp] GasConstants.Gbase
 -- We cannot prove full equivalence for the `EVM.step` function
 -- This is because it doesn't include all semantics such as gas computation
 theorem step_oneOp_equiv
-  {GAS_CELL ID_CELL ORIGIN_CELL CALLER_CELL COINBASE_CELL PC_CELL _Val0 _Val2 _Val6 _Val7 _Val8 : SortInt}
+  {GAS_CELL ID_CELL ORIGIN_CELL CALLER_CELL COINBASE_CELL TIMESTAMP_CELL PC_CELL _Val0 _Val2 _Val6 _Val7 _Val8 : SortInt}
   -- We assume `GASPRICE_CELL` is not negative
   {GASPRICE_CELL : ℕ}
   {SCHEDULE_CELL : SortSchedule}
@@ -433,16 +441,18 @@ theorem step_oneOp_equiv
   (CALLER_CELL_small : CALLER_CELL < AccountAddress.size)
   (CALLER_CELL_nonneg : 0 ≤ CALLER_CELL)
   (COINBASE_CELL_small : COINBASE_CELL < AccountAddress.size)
-  (COINBASE_CELL_nonneg : 0 ≤ COINBASE_CELL) :
-  let lhs := (@oneOpLHS op GAS_CELL ID_CELL ORIGIN_CELL CALLER_CELL COINBASE_CELL PC_CELL _Val6 _Val8 GASPRICE_CELL SCHEDULE_CELL USEGAS_CELL WS _DotVar0 _DotVar2 _Gen0 _Gen1 _Gen10
+  (COINBASE_CELL_nonneg : 0 ≤ COINBASE_CELL)
+  (TIMESTAMP_CELL_small : TIMESTAMP_CELL < UInt256.size)
+  (TIMESTAMP_CELL_nonneg : 0 ≤ TIMESTAMP_CELL) :
+  let lhs := (@oneOpLHS op GAS_CELL ID_CELL ORIGIN_CELL CALLER_CELL COINBASE_CELL TIMESTAMP_CELL PC_CELL _Val6 _Val8 GASPRICE_CELL SCHEDULE_CELL USEGAS_CELL WS _DotVar0 _DotVar2 _Gen0 _Gen1 _Gen10
   _Gen11 _Gen12 _Gen13 _Gen14 _Gen15 _Gen16 _Gen19
   _Gen20 _Gen21 _Gen22 _Gen3 _Gen4 _Gen5 _Gen6 _Gen7 _Gen8 _Gen9 _K_CELL)
-  let rhs := (@oneOpRHS (op.do lhs) ID_CELL ORIGIN_CELL CALLER_CELL COINBASE_CELL _Val6 _Val8 GASPRICE_CELL SCHEDULE_CELL WS _DotVar0 _DotVar2 _Gen0 _Gen1 _Gen10 _Gen11 _Gen12 _Gen13 _Gen14 _Gen15 _Gen16  _Gen19 _Gen20 _Gen21 _Gen22 _Gen3 _Gen4 _Gen5 _Gen6 _Gen7 _Gen8 _Gen9 _K_CELL)
+  let rhs := (@oneOpRHS (op.do lhs) ID_CELL ORIGIN_CELL CALLER_CELL COINBASE_CELL TIMESTAMP_CELL _Val6 _Val8 GASPRICE_CELL SCHEDULE_CELL WS _DotVar0 _DotVar2 _Gen0 _Gen1 _Gen10 _Gen11 _Gen12 _Gen13 _Gen14 _Gen15 _Gen16  _Gen19 _Gen20 _Gen21 _Gen22 _Gen3 _Gen4 _Gen5 _Gen6 _Gen7 _Gen8 _Gen9 _K_CELL)
   EVM.step_arith op.from_k gas gasCost (stateMap symState lhs) =
   .ok (stateMap {symState with execLength := symState.execLength + 1} rhs) := by
   intro lhs rhs
   rw [oneOp_prestate_equiv]
-  rw [@oneOp_poststate_equiv _ ID_CELL ORIGIN_CELL CALLER_CELL COINBASE_CELL PC_CELL]
+  rw [@oneOp_poststate_equiv _ ID_CELL ORIGIN_CELL CALLER_CELL COINBASE_CELL TIMESTAMP_CELL PC_CELL]
   <;> try assumption
   cases gas; contradiction
   case succ gas =>
@@ -458,7 +468,7 @@ theorem step_oneOp_equiv
        -- `address`
         simp [intMap, AccountAddress.ofNat, UInt256.ofNat, Id.run, UInt256.toSigned] <;>
         cases top_stack <;>
-        aesop (add simp [Fin.val, Fin.ofNat, AccountAddress.size, State.coinBase])
+        aesop (add simp [Fin.val, Fin.ofNat, AccountAddress.size, State.coinBase, State.timeStamp])
         (add safe (by omega))
       /- . -- `origin`
         simp [intMap, AccountAddress.ofNat, UInt256.ofNat, Id.run, UInt256.toSigned]
@@ -478,7 +488,7 @@ attribute [local simp] GasConstants.Glow
  6. `W0` and `W1` are nonnegative
  -/
 theorem X_oneOp_equiv
-  {GAS_CELL ID_CELL ORIGIN_CELL CALLER_CELL COINBASE_CELL PC_CELL _Val0 _Val2 _Val6 _Val7 _Val8 : SortInt}
+  {GAS_CELL ID_CELL ORIGIN_CELL CALLER_CELL COINBASE_CELL TIMESTAMP_CELL PC_CELL _Val0 _Val2 _Val6 _Val7 _Val8 : SortInt}
   -- We assume `GASPRICE_CELL` is not negative
   {GASPRICE_CELL : ℕ}
   {SCHEDULE_CELL : SortSchedule}
@@ -533,18 +543,21 @@ theorem X_oneOp_equiv
   (CALLER_CELL_small : CALLER_CELL < AccountAddress.size)
   (CALLER_CELL_nonneg : 0 ≤ CALLER_CELL)
   (COINBASE_CELL_small : COINBASE_CELL < AccountAddress.size)
-  (COINBASE_CELL_nonneg : 0 ≤ COINBASE_CELL) :
-  let lhs := (@oneOpLHS op GAS_CELL ID_CELL ORIGIN_CELL CALLER_CELL COINBASE_CELL PC_CELL _Val6 _Val8 GASPRICE_CELL SCHEDULE_CELL USEGAS_CELL WS _DotVar0 _DotVar2 ⟨op.from_k.to_bin⟩ _Gen1 _Gen10
+  (COINBASE_CELL_nonneg : 0 ≤ COINBASE_CELL)
+  (TIMESTAMP_CELL_small : TIMESTAMP_CELL < UInt256.size)
+  (TIMESTAMP_CELL_nonneg : 0 ≤ TIMESTAMP_CELL) :
+  let lhs := (@oneOpLHS op GAS_CELL ID_CELL ORIGIN_CELL CALLER_CELL COINBASE_CELL TIMESTAMP_CELL PC_CELL _Val6 _Val8 GASPRICE_CELL SCHEDULE_CELL USEGAS_CELL WS _DotVar0 _DotVar2 ⟨op.from_k.to_bin⟩ _Gen1 _Gen10
   _Gen11 _Gen12 _Gen13 _Gen14 _Gen15 _Gen16 _Gen19
   _Gen20 _Gen21 _Gen22 _Gen3 _Gen4 _Gen5 _Gen6 _Gen7 _Gen8 _Gen9 _K_CELL)
-  let rhs := (@oneOpRHS (op.do lhs) ID_CELL ORIGIN_CELL CALLER_CELL COINBASE_CELL _Val6 _Val8 GASPRICE_CELL SCHEDULE_CELL WS _DotVar0 _DotVar2 _Gen0 _Gen1 ⟨.empty⟩ _Gen11 _Gen12 _Gen13 _Gen14 _Gen15 _Gen16 _Gen19 _Gen20 _Gen21 _Gen22 _Gen3 _Gen4 _Gen5 _Gen6 _Gen7 _Gen8 _Gen9 _K_CELL)
+  let rhs := (@oneOpRHS (op.do lhs) ID_CELL ORIGIN_CELL CALLER_CELL COINBASE_CELL TIMESTAMP_CELL _Val6 _Val8 GASPRICE_CELL SCHEDULE_CELL WS _DotVar0 _DotVar2 _Gen0 _Gen1 ⟨.empty⟩ _Gen11 _Gen12 _Gen13 _Gen14 _Gen15 _Gen16 _Gen19 _Gen20 _Gen21 _Gen22 _Gen3 _Gen4 _Gen5 _Gen6 _Gen7 _Gen8 _Gen9 _K_CELL)
   EVM.X (UInt256.toNat (intMap GAS_CELL)) symValidJumps
   (stateMap symState lhs) =
   .ok (.success (stateMap {symState with execLength := symState.execLength + 2} rhs) ByteArray.empty) := by
   intro lhs rhs; simp [lhs, rhs]
   -- With `simp` doesn't work
   --rw [codeDiv, pcZero]
-  rw [oneOp_prestate_equiv, @oneOp_poststate_equiv _ ID_CELL ORIGIN_CELL CALLER_CELL COINBASE_CELL PC_CELL]
+  rw [oneOp_prestate_equiv]
+  rw [@oneOp_poststate_equiv _ ID_CELL ORIGIN_CELL CALLER_CELL COINBASE_CELL TIMESTAMP_CELL PC_CELL]
   <;> try assumption
   -- If we don't apply this lemma we cannot rewrite X_add_summary
   have pc_equiv : intMap 0 = UInt256.ofNat 0 := rfl
